project/encoding.v
@@ -27,29 +27,29 @@ Fixpoint findRef (n : nat) (refs : List.list (nat * nat)) :=
 
 Fixpoint encode (s : term) (u r : nat) (refs : List.list (nat * nat)) :=
   match s with
-  | Val v => encode_value v u refs
+  | Val v => Res (Out (u+1) 0 (encode_value v (incRefs 0 1 refs)))
   | Abs s => In u (In 0 (In 1 (In 2 (encode s 2 1 (List.cons (0,0) (incRefs 1 4 (refs)))))))
   | App s v => Res (Res (Par 
       (encode s 1 0 (incRefs 0 2 refs)) 
       (Res (Out 2 0 (Out 0 (u + 3) (Out 0 (r + 3) 
-        (encode_value v 0 (incRefs 0 3 refs))
+        ( ( Res (Out (u+4) 0 (encode_value v (incRefs 0 4 refs) ))))
       ))))
     ))
   | Force v => Res (Par 
-      (encode_value v 0 (incRefs 0 1 refs)) 
+      (Res ( Out (u+2) 0(encode_value v (incRefs 0 1 refs)) ))
       (In 0 (Res (Out 1 0 (Out 0 (u + 3) (Out 0 (r + 3) (Nil))))))
     )
-  | Ret v => encode_value v r refs
+  | Ret v => (Res (Out (r+1) 0 (encode_value v (incRefs 0 1 refs))))
   | Bind s t => Res (Par 
       (Res (encode s 0 1 (incRefs 0 2 refs))) 
       (In 0 (encode t (u + 2) (r + 2) (List.cons (0,0)(incRefs 1 2 refs))))
     )
   end
 
-with encode_value (v : value) (u : nat) (refs : List.list (nat * nat)) :=
+with encode_value (v : value) (refs : List.list (nat * nat)) :=
   match v with
-  | Var n => Res (Out (u + 1) 0 (Rep (In 0 (Out ((findRef n refs) + 2) 0 Nil))))
-  | Thunk s => Res (Out (u + 1) 0 (Rep (In 0 (In 0 (In 1 
-      (encode s 1 0 (incRefs 0 4 refs))
-    )))))
+  | Var n => Rep (In 0 (Out ((findRef n refs) + 1) 0 Nil))
+  | Thunk s => (Rep (In 0 (In 0 (In 1 
+      (encode s 1 0 (incRefs 0 3 refs))
+    ))))
   end.
