project/op_correspond.v
@@ -7,14 +7,50 @@ Require Coq.Lists.List.
 Require Import Nat.
 Require Coq.Lists.List.
 
+Lemma res_prefix_in : forall (P : proc) (V : value) (n: nat) (ref : List.list (nat * nat)),
+  Res(Par (In n P) (encode_value V ref)) ~~ In n (Res(Par (P) (encode_value V ref))).
+Proof. Admitted.
+
+Lemma res_prefix_out : forall (P : proc) (V : value) (n m: nat) (ref : List.list (nat * nat)),
+ ~(m = 0) -> (Res(Par (Out n m P) (encode_value V ref)) ~~ In n (Res(Par (P) (encode_value V ref)))).
+Proof. Admitted.
+
+Lemma pointer : forall (P Q : proc) (x y : nat) (V : value) (ref : List.list (nat * nat)),
+  Res (Par (Par (P) (Q)) (encode_value V ref)) ~~ 
+  Res (Res (Par 
+            (Par ((P[[shift]])[[swap]]) (Q[[shift]]) ) 
+            (Par (((encode_value V (incRefs 0 1 ref))[[shift]])[[swap]]) ((encode_value V (incRefs 0 1 ref))[[shift]])))).
+Proof. Admitted.
+
+Lemma res_rep : forall (P : proc) (V : value) (ref : List.list (nat * nat)),
+Res( Par (Rep (P)) (encode_value V ref) ) ~~ Rep (Res (Par (P) (encode_value V ref))).
+Proof. Admitted.
+
+Lemma sub_lemma : forall (M : term) (V : value) (u r : nat) (ref : List.list (nat * nat)),
+encode (M [l[(extend_subst_lam V Var)]l]) u r ref ~~ Res ( Par ((encode M (u+1) (r+1) (incRefs 0 1 ref))) (encode_value V ref)).  
+Proof. Admitted.
 
 Theorem Sound_encoding : 
 forall (M N : term) (u r : nat), M --> N -> (exists (P' : proc), (encode M u r List.nil) =(a_tau)> P' 
   /\ (P' ~~ (encode N u r List.nil))). 
 Proof. intros. induction H.
   - simpl.
-  induction v.
+  induction v. 
   * simpl.
+  exists (Res(Res(
+    (Par
+       (Res
+          
+             ((Rep (In 0 (Out (n + 1) 0 Nil))[[swap]])))
+       (
+          (encode s (u + 2) (r + 2)
+             ((0, 0) :: Datatypes.nil)[[0 |> id]])))))).
+    split.
+    + apply ACTION. apply RES22. apply COM22 with (n := 0).
+      apply RESBOUT. apply RES1. apply OUT.
+      apply IN.
+    +
+
   Admitted.
 
 Theorem Complete_encoding : 
